Loda/TypingTest.lean
@@ -5,20 +5,21 @@ open Ast
 
 -- dummy environments
 def σ0 : Env := fun _ => Value.vBool true
-def Γ0 : TyEnv := fun _ => (Ty.refin Ty.bool (True))
+def Γ0 : TyEnv := fun _ => (Ty.refin Ty.bool (Ast.Expr.constBool true))
 def Γ1 := setTy Γ0 "x" Ty.bool
 def δ0 : Ast.CircuitEnv :=
   fun _ => { name := "idInt", inputs := [("x", Ast.Ty.int)], output := Ast.Ty.int,
                  body := Ast.Expr.var "x" }
 
-example : SubtypeJudgment σ0 Γ0 (pure Ty.int) (pure Ty.int) :=
+example : SubtypeJudgment σ0 δ0 Γ0 123 (pure Ty.int) (pure Ty.int) :=
   SubtypeJudgment.TSub_Refl
 
 -- refinement subtyping: {v:int | True} <: {v:int | True}
-example : SubtypeJudgment σ0 Γ0 (pure (Ty.refin Ty.int True)) (pure (Ty.refin Ty.int True)) := by
+example : SubtypeJudgment σ0 δ0 Γ0 123 (pure (Ty.refin Ty.int (Ast.Expr.constBool true))) (pure (Ty.refin Ty.int (Ast.Expr.constBool true))) := by
   apply SubtypeJudgment.TSub_Refl
 
 -- TE_VAR: assume env maps "b" to {v | v = eval ...}
-example : TypeJudgment σ0 δ0 Γ0 123 (Expr.var "b") ((Ty.refin Ty.bool (Value.vBool true = σ0 "b")), σ0) := by
+example : TypeJudgment σ0 δ0 Γ0 123 (Expr.var "b") ((Ty.refin Ty.bool (eeq v (Ast.Expr.var "b"))), σ0) := by
   apply TypeJudgment.TE_Var
   simp [Γ0]
+  rfl
